Explicit_sub.v
@@ -1,0 +1,79 @@
+Require Export TheoryInTerm.
+
+Import BuildModel.
+Import CCM.
+Import IZF.
+Import T J.
+
+Definition esub := {f : val->val | Proper (eq_val ==> eq_val) f}.
+
+Definition eq_esub es es':= 
+  forall i i', eq_val i i' -> eq_val (es i) (es' i).
+
+Definition esub_conv (f : esub) (es : val) := proj1_sig f es.
+
+Instance esub_conv_morph : Proper (eq ==> eq_val ==> eq_val) esub_conv.
+do 4 red; simpl; intros. subst y.
+destruct x; simpl. rewrite H0; reflexivity.
+Qed.
+
+Definition app_esub : esub -> term -> term.
+intros es t. left. 
+exists (fun i => int t (esub_conv es i)).
+do 3 red; intros. apply int_morph; try reflexivity.
+ apply esub_conv_morph; trivial.
+Defined.
+
+Definition id_sub : esub.
+exists (fun f => f). do 2 red; trivial.
+Defined.
+
+Definition sub_cons : term -> esub -> esub.
+intros t es.
+exists (fun i => V.cons (int t i) (esub_conv es i)).
+do 2 red; intros. apply V.cons_morph; 
+  [rewrite H; reflexivity| apply esub_conv_morph; trivial].
+Defined.
+
+Definition typ_esub env1 es env2 := forall i, 
+  val_ok env1 i -> val_ok env2 (esub_conv es i).
+
+Lemma esub_typ_id : forall env, typ_esub env id_sub nil.
+do 2 red; intros. destruct n; simpl in H0; discriminate.
+Qed.
+
+Lemma esub_typ_cons : forall env1 env2 s t A,
+  typ_esub env1 s env2 ->
+  typ env1 t (app_esub s A) ->
+  typ_esub env1 (sub_cons t s) (A::env2).
+red; intros. simpl. 
+apply vcons_add_var; [apply H | apply H0]; trivial.
+Qed.
+
+Lemma explicit_sub : forall env1 env2 s t A, A <> None ->
+  typ_esub env1 s env2 ->
+  typ env2 t A -> 
+  typ env1 (app_esub s t) (app_esub s A).
+do 2 red; simpl; intros.
+red in H0; specialize H0 with (1:=H2).
+do 2 red in H1. specialize H1 with (1:=H0).
+destruct A; trivial.
+ elim H; trivial.
+Qed.
+
+Lemma EQ_trm_esub : forall x y s, 
+  eq_term (app_esub s (EQ_trm x y)) (EQ_trm (app_esub s x) (app_esub s y)).
+red; simpl; red; intros. 
+replace (fun k : nat => esub_conv s x0 k) with (esub_conv s x0); trivial.
+replace (esub_conv s (fun k : nat => y0 k)) with (esub_conv s y0); trivial.
+apply ZFind_basic.EQ_morph; [|rewrite H|rewrite H]; reflexivity.
+Qed.
+
+Definition eq_fosub n' e s s' := forall n, n < n' ->
+  eq_typ e (app_esub s (Ref n)) (app_esub s' (Ref n)) /\
+  typ e (app_esub s (Ref n)) T /\ typ e (app_esub s' (Ref n)) T.
+
+
+
+
+  
