basic1.v
@@ -1,0 +1,37 @@
+Require Import Omega.
+
+Lemma succ_max_distr : forall n m, S (max n m) = max (S n) (S m).
+induction n; destruct m; simpl; reflexivity.
+Qed.
+
+Lemma max_split1 : forall x y z, z < x -> z < max x y.
+induction x; simpl; intros.
+ apply False_ind; omega.
+
+ destruct y; trivial.
+  destruct z; try omega.
+   assert (z < x) by omega. specialize IHx with (1:=H0) (y:=y). omega.
+Qed.
+
+Lemma max_split2 : forall x y z, z < y -> z < max x y.
+induction x; simpl; intros; trivial.
+ destruct y; trivial.
+  apply False_ind; omega.
+ 
+  destruct z; try omega.
+   assert (z < y) by omega. specialize IHx with (1:=H0). omega.
+Qed.
+
+Lemma max_comb : forall x y z, z < max x y -> z < x \/ z < y.
+induction x; simpl; intros.
+ right; trivial.
+
+ destruct y.
+  left; trivial.
+
+  destruct z.
+   left; omega.
+
+   assert (z < max x y) by omega.
+   specialize IHx with (1:=H0). destruct IHx; [left | right]; omega.
+Qed.
